some steps towards arith tactic

ulib/FStar.Reflection.Arith.fst
@@ -22,28 +22,31 @@ type expr =
     | Atom : nat -> expr // uninterpreted atom
 
 type connective =
-    | Lt | Eq | Gt | Ne
+    | C_Lt | C_Eq | C_Gt | C_Ne
 
-type prop = | MkProp : expr ->  connective -> expr -> prop
+type prop =
+    | CompProp : expr -> connective -> expr -> prop
+    | AndProp  : prop -> prop -> prop
+    | OrProp   : prop -> prop -> prop
 
-let lt e1 e2 = MkProp e1 Lt e2
-let le e1 e2 = MkProp e1 Lt (Plus (Lit 1) e2)
-let eq e1 e2 = MkProp e1 Eq e2
-let ne e1 e2 = MkProp e1 Ne e2
-let gt e1 e2 = MkProp e1 Gt e2
-let ge e1 e2 = MkProp (Plus (Lit 1) e1) Gt e2
+let lt e1 e2 = CompProp e1 C_Lt e2
+let le e1 e2 = CompProp e1 C_Lt (Plus (Lit 1) e2)
+let eq e1 e2 = CompProp e1 C_Eq e2
+let ne e1 e2 = CompProp e1 C_Ne e2
+let gt e1 e2 = CompProp e1 C_Gt e2
+let ge e1 e2 = CompProp (Plus (Lit 1) e1) C_Gt e2
 
 (* Define a traversal monad! Makes exception handling and counter-keeping easy *)
-let tm a = nat -> option (a * nat)
-let return (x:'a) : tm 'a = fun i -> Some (x, i)
-let bind (m : tm 'a) (f : 'a -> tm 'b) : tm 'b =
+private let tm a = nat -> option (a * nat)
+private let return (x:'a) : tm 'a = fun i -> Some (x, i)
+private let bind (m : tm 'a) (f : 'a -> tm 'b) : tm 'b =
     fun i -> match m i with
              | Some (x, j) -> f x j
              | None -> None
 
-let atom : tm nat = fun i -> Some (i, i + 1)
-val fail : (#a:Type) -> tm a
-let fail #a = fun i -> None
+private let atom : tm nat = fun i -> Some (i, i + 1)
+private val fail : (#a:Type) -> tm a
+private let fail #a = fun i -> None
 
 let rec forall_list (p:'a -> Type) (l:list 'a) : Type =
     match l with
@@ -63,8 +66,8 @@ let liftM2 f x y =
 
 let minus x y = Plus x (Neg y)
 
-val decide : term -> tm expr
-let rec decide (t:term) =
+val is_arith_expr : term -> tm expr
+let rec is_arith_expr (t:term) =
     let hd, tl = collect_app t in
     match inspect hd, tl with
     | Tv_FVar fv, [l; r] ->
@@ -72,8 +75,8 @@ let rec decide (t:term) =
         collect_app_order t;
         // Have to go through hoops to get F* to typecheck this.
         // Maybe the do notation is twisting the terms somehow unexpected?
-        let ll = decide (l <: x:term{x << t}) in
-        let rr = decide (r <: x:term{x << t}) in
+        let ll = is_arith_expr (l <: x:term{x << t}) in
+        let rr = is_arith_expr (r <: x:term{x << t}) in
         if      eq_qn qn add_qn   then liftM2 Plus ll rr
         else if eq_qn qn minus_qn then liftM2 minus ll rr
         else if eq_qn qn mult_qn  then liftM2 Mult ll rr
@@ -81,7 +84,7 @@ let rec decide (t:term) =
     | Tv_FVar fv, [a] ->
         let qn = inspect_fv fv in
         collect_app_order t;
-        let aa = decide (a <: x:term{x << t}) in
+        let aa = is_arith_expr (a <: x:term{x << t}) in
         if   eq_qn qn neg_qn then liftM Neg aa
         else fail
     | Tv_Const (C_Int i), _ ->
@@ -89,12 +92,19 @@ let rec decide (t:term) =
     | _, _ ->
         fail
 
+val is_arith_prop : term -> tm prop
+let rec is_arith_prop (t:term) =
+    match term_as_formula t with
+    | Eq _ l r -> liftM2 eq (is_arith_expr l) (is_arith_expr r)
+    | And l r  -> liftM2 AndProp (is_arith_prop l) (is_arith_prop r)
+    | Or l r   -> liftM2  OrProp (is_arith_prop l) (is_arith_prop r)
+    | _ -> fail
 
 let test =
     let bind = FStar.Tactics.bind in
     let fail = FStar.Tactics.fail in
     assert_by_tactic (t <-- quote (1 + 2);
-                             match decide t 0 with
+                             match is_arith_expr t 0 with
                              | Some (Plus (Lit 1) (Lit 2), _) -> print "alright!"
                              | _ -> fail "oops")
                             True
