examples/tactics/Arith.fst
@@ -1,0 +1,52 @@
+module Arith
+
+// Testing out an arithmetic tactic.
+
+open FStar.Tactics
+open FStar.Reflection.Arith
+open FStar.List
+
+// decide if the current goal is arith
+let is_arith_goal : tactic bool =
+    eg <-- cur_goal;
+    let _, g = eg in
+    match is_arith_prop g 0 with
+    | Some _ -> return true
+    | None -> return false
+
+
+val split_arith : unit -> Tac unit
+let rec split_arith = fun () -> (
+    addns ["Blah"];;
+    prune [];;
+    b <-- is_arith_goal;
+    if b then (
+        addns ["Prims"];;
+        smt
+    ) else (
+        eg <-- cur_goal;
+        let _, g = eg in
+        match term_as_formula g with
+        | True_ -> trivial
+        //| And l r -> seq FStar.Tactics.split split_arith
+        | _ -> return ()
+    )) ()
+    
+
+// TODO: even if encoding this module to SMT, x is not given a HasType
+assume val x : int
+
+let _ = assert_by_tactic (prune [];;
+                          FStar.Tactics.split;;
+                          (* rev part *)
+                            addns ["FStar";"List"];;
+                            addns ["Prims"];;
+                            smt;;
+                          (* arithmetic part *)
+                            addns ["Prims"];;
+                            addns ["Arith"];;
+                            smt;;
+                          return ()
+                         )
+                         (FStar.List.Tot.rev [1;2;3;4] == [4;3;2;1]
+                            /\ op_Multiply 2 (x + 3) == 6 + (op_Multiply 3 x) - x)
